src/Ast/Resolver.dfy
@@ -8,6 +8,7 @@ module Resolver {
   import opened Types
   import Raw = RawAst
   import opened Ast
+  import Printer
 
   method Resolve(b3: Raw.Program) returns (r: Result<Ast.Program, string>)
     ensures r.Success? ==> b3.WellFormed() && r.value.WellFormed()
@@ -36,23 +37,33 @@ module Resolver {
 
     var procMap: map<string, Procedure> := map[];
     for n := 0 to |b3.procedures|
-      // procMap maps the user-defined procedures seen so far to distinct procedure-declaration objects
+      // procMap maps the user-defined procedures seen so far to distinct and fresh procedure-declaration objects
       invariant procMap.Keys == set proc <- b3.procedures[..n] :: proc.name
       invariant MapIsInjective(procMap)
+      invariant forall name <- procMap :: fresh(procMap[name])
       // procMap organizes procedure-declaration objects correctly according to their names
       invariant forall procname <- procMap.Keys :: procMap[procname].Name == procname
       // user-defined types seen so far have distinct names
       invariant forall i, j :: 0 <= i < j < n ==> b3.procedures[i].name != b3.procedures[j].name
       // the procedures seen so far are well-formed
-      invariant forall proc <- b3.procedures[..n] :: proc.WellFormed(b3)
+      invariant forall proc <- b3.procedures[..n] :: proc.SignatureWellFormed(b3) && procMap[proc.name].SignatureWellFormed(proc)
     {
       var proc := b3.procedures[n];
       var name := proc.name;
       if name in procMap.Keys {
         return Failure("duplicate procedure name: " + name);
       }
-      var rproc :- ResolveProcedure(proc, b3);
+      var rproc :- ResolveProcedureSignature(proc, b3, typeMap);
       procMap := procMap[name := rproc];
+    }
+
+    var rs := ResolverState(b3, typeMap, procMap);
+    for n := 0 to |b3.procedures|
+      invariant forall proc <- b3.procedures :: proc.SignatureWellFormed(b3) && procMap[proc.name].SignatureWellFormed(proc)
+      invariant forall proc <- b3.procedures[..n] :: proc.WellFormed(b3)
+    {
+      var proc := b3.procedures[n];
+      var _ :- ResolveProcedure(proc, procMap[proc.name], rs);
     }
 
     var r3 := Program(typeMap.Values, procMap.Values);
@@ -60,48 +71,383 @@ module Resolver {
     return Success(r3);
   }
 
-  method ResolveProcedure(proc: Raw.Procedure, b3: Raw.Program) returns (r: Result<Procedure, string>)
-    ensures r.Success? ==> proc.WellFormed(b3)
-    ensures r.Success? ==> r.value.Name == proc.name
+  method ResolveProcedureSignature(proc: Raw.Procedure, b3: Raw.Program, typeMap: map<string, Type>) returns (r: Result<Procedure, string>)
+    requires forall typename :: b3.IsType(typename) <==> typename in typeMap
+    ensures r.Success? ==> proc.SignatureWellFormed(b3)
+    ensures r.Success? ==> fresh(r.value) && r.value.SignatureWellFormed(proc)
   {
-    if p :| p in proc.parameters && !Raw.LegalVariableName(p.name, {}) {
-      return Failure("illegal parameter name: " + p.name);
+    var paramMap: map<string, Variable> := map[];
+    var formals: seq<Parameter> := [];
+    for n := 0 to |proc.parameters|
+      invariant forall p <- proc.parameters[..n] :: Raw.LegalVariableName(p.name, {}) && b3.IsType(p.typ)
+      invariant forall i, j :: 0 <= i < j < n ==> proc.parameters[i].name != proc.parameters[j].name
+      invariant paramMap.Keys ==
+        (set p <- proc.parameters[..n] :: p.name) +
+        (set p <- proc.parameters[..n] | p.mode == Raw.InOut :: Raw.OldName(p.name))
+      invariant |formals| == n
+      invariant forall i :: 0 <= i < n ==> formals[i] == paramMap[proc.parameters[i].name]
+      invariant forall i :: 0 <= i < n ==> formals[i].name == proc.parameters[i].name
+      invariant forall i :: 0 <= i < n ==> formals[i].mode == proc.parameters[i].mode
+      invariant forall i :: 0 <= i < n ==> (formals[i].oldInOut.Some? <==> proc.parameters[i].mode == Raw.InOut)
+    {
+      var p := proc.parameters[n];
+      if !Raw.LegalVariableName(p.name, {}) {
+        return Failure("illegal parameter name: " + p.name);
+      }
+      if p.name in paramMap {
+        return Failure("duplicate parameter name: " + p.name);
+      }
+      var typ :- ResolveType(p.typ, typeMap);
+
+      var oldInOut;
+      if p.mode == Raw.InOut {
+        var v := new LocalVariable(Raw.OldName(p.name), false, typ);
+        oldInOut := Some(v);
+        paramMap := paramMap[Raw.OldName(p.name) := v];
+      } else {
+        oldInOut := None;
+      }
+
+      var formal := new Parameter(p.name, p.mode, typ, oldInOut);
+      paramMap := paramMap[p.name := formal];
+      formals := formals + [formal];
     }
 
-    if p :| p in proc.parameters && !b3.IsType(p.typ) {
-      return Failure("unknown type: " + p.typ);
+    var rproc := new Procedure(proc.name, formals);
+    return Success(rproc);
+  }
+
+  method ResolveType(typename: string, typeMap: map<string, Type>) returns (r: Result<Type, string>)
+    ensures r.Success? ==> typename in typeMap
+  {
+    if typename !in typeMap {
+      return Failure("unknown type: " + typename);
+    }
+    return Success(typeMap[typename]);
+  }
+
+  datatype ResolverState = ResolverState(b3: Raw.Program, typeMap: map<string, Type>, procMap: map<string, Procedure>)
+  {
+    ghost predicate Valid() {
+      && (forall typename :: b3.IsType(typename) <==> typename in typeMap)
+      && (forall procname <- procMap :: exists proc <- b3.procedures :: proc.name == procname)
+      && (forall rawProc <- b3.procedures ::
+            rawProc.name in procMap &&
+            var proc := procMap[rawProc.name];
+            && |rawProc.parameters| == |proc.Parameters|
+            && (forall i :: 0 <= i < |rawProc.parameters| ==> rawProc.parameters[i].mode == proc.Parameters[i].mode)
+         )
+    }
+  }
+
+  datatype LocalResolverState = LocalResolverState(
+    varMap: map<string, Variable>,
+    labelMap: map<string, Label>,
+    loopLabel: Option<Label>,
+    returnLabel: Label)
+  {
+    function AddVariable(name: string, v: Variable): LocalResolverState
+      ensures AddVariable(name, v).varMap.Keys == varMap.Keys + {name}
+    {
+      this.(varMap := varMap[name := v])
     }
 
-    if i, j :| 0 <= i < j < |proc.parameters| && proc.parameters[i].name == proc.parameters[j].name {
-      return Failure("duplicate parameter name: " + proc.parameters[i].name);
+    function FindLabel(name: string): Result<Label, string> {
+      if name in labelMap then
+        Success(labelMap[name])
+      else
+        Failure("undeclared exit label: " + name)
     }
+
+    function LabelSet(): set<string>
+      ensures labelMap == map[] ==> LabelSet() == {}
+    {
+      labelMap.Keys
+    }
+
+    function AddLabel(name: string, lbl: Label): LocalResolverState
+      ensures AddLabel(name, lbl).labelMap.Keys == labelMap.Keys + {name}
+    {
+      this.(labelMap := labelMap[name := lbl])
+    }
+
+    method GenerateLoopLabel() returns (lbl: Label, ls: LocalResolverState)
+      ensures ls.varMap.Keys == varMap.Keys
+      ensures ls.LabelSet() == LabelSet()
+      ensures ls.loopLabel.Some?
+    {
+      lbl := new Label("loop");
+      ls := this.(loopLabel := Some(lbl));
+    }
+  }
+
+  method ResolveProcedure(proc: Raw.Procedure, rproc: Procedure, rs: ResolverState) returns (r: Result<(), string>)
+    requires proc.SignatureWellFormed(rs.b3) && rproc.SignatureWellFormed(proc) && rs.Valid()
+    modifies rproc
+    ensures r.Success? ==> proc.WellFormed(rs.b3)
+  {
+    var formals := rproc.Parameters;
+    var n := |formals|;
+    assert forall formal: Parameter <- formals :: Raw.LegalVariableName(formal.name, {});
+    assert forall i, j :: 0 <= i < j < n ==> formals[i].name != formals[j].name;
+    forall i, j | 0 <= i < j < n
+      ensures Raw.OldName(formals[i].name) != Raw.OldName(formals[j].name)
+    {
+      var a, b := formals[i].name, formals[j].name;
+      assert a != b;
+      assert Raw.OldName(a)[|Raw.OldPrefix|..] == a;
+      assert Raw.OldName(a) != Raw.OldName(b);
+    }
+    var paramMap :=
+      (map formal <- rproc.Parameters :: formal.name := formal) +
+      (map formal <- rproc.Parameters | formal.oldInOut.Some? :: Raw.OldName(formal.name) := formal.oldInOut.value);
+
+    assert n == |proc.parameters|;
+    assert forall i :: 0 <= i < n ==> formals[i].name == proc.parameters[i].name;
+    assert forall i :: 0 <= i < n ==> (formals[i].oldInOut.Some? <==> proc.parameters[i].mode == Raw.InOut);
 
     var preScope := set p <- proc.parameters | p.mode.IsIncoming() :: p.name;
-    var bodyScope := set p <- proc.parameters :: p.name;
-    var postScope := bodyScope + (set p <- proc.parameters | p.mode == Raw.InOut :: Raw.OldName(p.name));
+    var postScope := (set p <- proc.parameters :: p.name) + (set p <- proc.parameters | p.mode == Raw.InOut :: Raw.OldName(p.name));
 
-    if ae :| ae in proc.pre && !ae.WellFormed(b3, preScope) {
-      return Failure("ill-formed precondition of procedure " + proc.name);
+    var returnLabel := new Label("return");
+
+    var preVariables := MapProject(paramMap, preScope);
+    assert preVariables.Keys == preScope;
+    var pre :- ResolveAExprs(proc.pre, rs, LocalResolverState(preVariables, map[], None, returnLabel));
+
+    var postVariables := MapProject(paramMap, postScope);
+    assert postVariables.Keys == postScope;
+    var ls := LocalResolverState(postVariables, map[], None, returnLabel);
+    var post :- ResolveAExprs(proc.post, rs, ls);
+
+    var body;
+    if proc.body == None {
+      body := None;
+    } else {
+      var b :- ResolveStmt(proc.body.value, rs, ls);
+      body := Some(b);
     }
 
-    if ae :| ae in proc.post && !ae.WellFormed(b3, postScope) {
-      return Failure("ill-formed postcondition of procedure " + proc.name);
-    }
+    rproc.Pre := pre;
+    rproc.Post := post;
+    rproc.Body := body;
+    return Success(());
+  }
 
-    if proc.body.Some? {
-      if !proc.body.value.WellFormed(b3, bodyScope, {}, false) {
-        return Failure("ill-formed body of procedure " + proc.name);
+  method ResolveAExprs(aexprs: seq<Raw.AExpr>, rs: ResolverState, ls: LocalResolverState) returns (r: Result<seq<AExpr>, string>)
+    requires rs.Valid()
+    ensures r.Success? ==> forall ae <- aexprs :: ae.WellFormed(rs.b3, ls.varMap.Keys)
+  {
+    var result := [];
+    for n := 0 to |aexprs|
+      invariant forall ae <- aexprs[..n] :: ae.WellFormed(rs.b3, ls.varMap.Keys)
+    {
+      var ae :- ResolveAExpr(aexprs[n], rs, ls);
+      result := result + [ae];
+    }
+    return Success(result);
+  }
+
+  method ResolveAExpr(aexpr: Raw.AExpr, rs: ResolverState, ls: LocalResolverState) returns (r: Result<AExpr, string>)
+    requires rs.Valid()
+    ensures r.Success? ==> aexpr.WellFormed(rs.b3, ls.varMap.Keys)
+  {
+    match aexpr
+    case AExpr(e) =>
+      var expr :- ResolveExpr(e, rs, ls.varMap);
+      return Success(AExpr(expr));
+    case AAssertion(s) =>
+      var stmt :- ResolveStmt(s, rs, ls.(labelMap := map[], loopLabel := None));
+      return Success(AAssertion(stmt));
+  }
+
+  method ResolveStmt(stmt: Raw.Stmt, rs: ResolverState, ls: LocalResolverState) returns (result: Result<Stmt, string>)
+    requires rs.Valid()
+    ensures result.Success? ==> stmt.WellFormed(rs.b3, ls.varMap.Keys, ls.LabelSet(), ls.loopLabel.Some?)
+  {
+    var r: Stmt;
+    match stmt {
+      case VarDecl(variable, init, body) =>
+        if !Raw.LegalVariableName(variable.name, ls.varMap.Keys) {
+          return Failure("illegal variable name: " + variable.name);
+        }
+        var typ :- ResolveType(variable.typ, rs.typeMap);
+        var v := new LocalVariable(variable.name, variable.isMutable, typ);
+        var i;
+        if init == None {
+          i := None;
+        } else {
+          var e :- ResolveExpr(init.value, rs, ls.varMap);
+          i := Some(e);
+        }
+        var ls' := ls.AddVariable(variable.name, v);
+        assert ls'.varMap.Keys == ls.varMap.Keys + {v.name};
+        var b :- ResolveStmt(body, rs, ls');
+        r := VarDecl(v, i, b);
+
+      case Assign(lhs, rhs) =>
+        if lhs !in ls.varMap {
+          return Failure("undeclared variable: " + lhs);
+        }
+        var left := ls.varMap[lhs];
+        var right :- ResolveExpr(rhs, rs, ls.varMap);
+        r := Assign(left, right);
+
+      case Block(stmts) =>
+        var ss := [];
+        for n := 0 to |stmts|
+          invariant forall stmt <- stmts[..n] :: stmt.WellFormed(rs.b3, ls.varMap.Keys, ls.LabelSet(), ls.loopLabel.Some?)
+        {
+          var s :- ResolveStmt(stmts[n], rs, ls);
+          ss := ss + [s];
+        }
+        r := Block(ss);
+
+      case Call(_, _) =>
+        r :- ResolveCallStmt(stmt, rs, ls);
+
+      case Check(cond) =>
+        var c :- ResolveExpr(cond, rs, ls.varMap);
+        r := Check(c);
+
+      case Assume(cond) =>
+        var c :- ResolveExpr(cond, rs, ls.varMap);
+        r := Assume(c);
+
+      case Assert(cond) =>
+        var c :- ResolveExpr(cond, rs, ls.varMap);
+        r := Assert(c);
+
+      case AForall(name, typ, body) =>
+        if !Raw.LegalVariableName(name, ls.varMap.Keys) {
+          return Failure("illegal variable name: " + name);
+        }
+        var t :- ResolveType(typ, rs.typeMap);
+        var v := new LocalVariable(name, false, t);
+        var b :- ResolveStmt(body, rs, ls.AddVariable(name, v));
+        r := AForall(v, b);
+
+      case If(cond, thn, els) =>
+        var c :- ResolveExpr(cond, rs, ls.varMap);
+        var th :- ResolveStmt(thn, rs, ls);
+        var el :- ResolveStmt(els, rs, ls);
+        var case0 := Case(c, th);
+        var case1 := Case(Expr.CreateNegation(c), el);
+        r := If([case0, case1]);
+
+      case IfCase(cases) =>
+        if |cases| == 0 {
+          return Failure("an if-case statement must have at least 1 case");
+        }
+        var cc := [];
+        for n := 0 to |cases|
+          invariant forall cs <- cases[..n] ::
+            && cs.cond.WellFormed(rs.b3, ls.varMap.Keys)
+            && cs.body.WellFormed(rs.b3, ls.varMap.Keys, ls.LabelSet(), ls.loopLabel.Some?)
+        {
+          var cond :- ResolveExpr(cases[n].cond, rs, ls.varMap);
+          var body :- ResolveStmt(cases[n].body, rs, ls);
+          cc := cc + [Case(cond, body)];
+        }
+        r := If(cc);
+
+      case Loop(invariants, body) =>
+        var invs :- ResolveAExprs(invariants, rs, ls);
+        var loopLabel, ls' := ls.GenerateLoopLabel();
+        var b :- ResolveStmt(body, rs, ls');
+        r := LabeledStmt(loopLabel, Loop(invs, b));
+        assert stmt.WellFormed(rs.b3, ls.varMap.Keys, ls.LabelSet(), ls.loopLabel.Some?) by {
+          assert forall ae <- invariants :: ae.WellFormed(rs.b3, ls.varMap.Keys);
+          assert ls.varMap.Keys == ls'.varMap.Keys;
+          assert ls.LabelSet() == ls'.LabelSet();
+          assert ls'.loopLabel.Some?;
+          assert body.WellFormed(rs.b3, ls'.varMap.Keys, ls'.LabelSet(), ls'.loopLabel.Some?);
+        }
+
+      case LabeledStmt(lbl, body) =>
+        if lbl in ls.labelMap {
+          return Failure("duplicate label name: " + lbl);
+        }
+        var l := new Label(lbl);
+        var b :- ResolveStmt(body, rs, ls.AddLabel(lbl, l));
+        r := LabeledStmt(l, b);
+
+      case Exit(maybeLabel) =>
+        match maybeLabel {
+          case None =>
+            if ls.loopLabel == None {
+              return Failure("an 'exit' statement outside a loop requires a label");
+            }
+            r := Exit(ls.loopLabel.value);
+          case Some(name) =>
+            var lbl :- ls.FindLabel(name);
+            r := Exit(lbl);
+        }
+
+      case Return =>
+        r := Exit(ls.returnLabel);
+
+      case Probe(expr) =>
+        var e :- ResolveExpr(expr, rs, ls.varMap);
+        r := Probe(e);
+    }
+    return Success(r);
+  }
+
+  method ResolveCallStmt(stmt: Raw.Stmt, rs: ResolverState, ls: LocalResolverState) returns (result: Result<Stmt, string>)
+    requires stmt.Call? && rs.Valid()
+    ensures result.Success? ==> stmt.WellFormed(rs.b3, ls.varMap.Keys, ls.LabelSet(), ls.loopLabel.Some?)
+  {
+    var Call(name, args) := stmt;
+
+    if name !in rs.procMap {
+      return Failure("call to undeclared procedure: " + name);
+    }
+    var proc := rs.procMap[name];
+    var rawProc :| rawProc in rs.b3.procedures && rawProc.name == name;
+    assert |rawProc.parameters| == |proc.Parameters|;
+
+    if |args| != |proc.Parameters| {
+      return Failure("wrong number of arguments in call to procedure " + name);
+    }
+    assert |args| == |rawProc.parameters|;
+
+    var aa := [];
+    for n := 0 to |args|
+      invariant forall i :: 0 <= i < n ==> args[i].mode == rawProc.parameters[i].mode
+      invariant forall i :: 0 <= i < n ==> args[i].arg.WellFormed(rs.b3, ls.varMap.Keys)
+    {
+      if args[n].mode != proc.Parameters[n].mode {
+        return Failure("mismatched parameter mode in call to procedure " + name);
       }
+      var e :- ResolveExpr(args[n].arg, rs, ls.varMap);
+      var ca;
+      if args[n].mode == Raw.In {
+        ca := InArgument(e);
+      } else if !e.IdExpr? {
+        return Failure(Printer.ParameterMode(args[n].mode) + "argument must be a variable");
+      } else {
+        ca := OutgoingArgument(args[n].mode == Raw.InOut, e.v);
+      }
+      aa := aa + [ca];
     }
 
-    var rproc := new Procedure(proc.name, [], [], []); // TODO: other parameters
-    assert proc.WellFormed(b3) by {
-      assert forall p <- proc.parameters :: Raw.LegalVariableName(p.name, {}) && b3.IsType(p.typ);
-      assert Parameter.UniqueNames(proc.parameters);
-      assert forall ae <- proc.pre :: ae.WellFormed(b3, preScope);
-      assert forall ae <- proc.post :: ae.WellFormed(b3, postScope);
-      assert proc.body == None || proc.body.value.WellFormed(b3, bodyScope, {}, false);
+    return Success(Call(proc, aa));
+  }
+
+  method ResolveExpr(expr: Raw.Expr, rs: ResolverState, varMap: map<string, Variable>) returns (result: Result<Expr, string>)
+    ensures result.Success? ==> expr.WellFormed(rs.b3, varMap.Keys)
+  {
+    var r: Expr;
+    match expr {
+      case Const(value) =>
+        r := Const(value);
+      case IdExpr(name) =>
+        if name !in varMap {
+          return Failure("undeclared variable: " + name);
+        }
+        r := IdExpr(varMap[name]);
     }
-    return Success(rproc);
+    return Success(r);
   }
 }
